Resolve wishlist

theories/tree_borrows/wishlist.v
@@ -1,3 +1,6 @@
+(** Abstraction layer for trees.
+    The goal of this file is that lemmas that appear here expose as few internal details
+    as possible. In particular they should all refer to [trees] in their signature (NOT [tree]). *)
 From iris.proofmode Require Export proofmode.
 From iris.base_logic.lib Require Import ghost_map.
 From simuliris.base_logic Require Export gen_sim_prog.
@@ -9,18 +12,46 @@ From simuliris.tree_borrows Require Import steps_progress steps_retag steps_inv.
 From simuliris.tree_borrows Require Import logical_state inv_accessors.
 From iris.prelude Require Import options.
 
-
-
-Lemma trees_contain_trees_lookup tr ev1 ev2 blk tg :
-  wf_trees tr ev1 ev2 →
-  trees_contain tg tr blk → ∃ it, trees_lookup tr blk tg it.
+(***** not part of the API *****)
+Lemma trees_at_block_projection trs tr blk P :
+  trees_at_block P trs blk ->
+  trs !! blk = Some tr ->
+  P tr.
 Proof.
-Admitted.
+  rewrite /trees_contain /trees_at_block.
+  destruct (trs !! blk); [|tauto].
+  intros Ex Eq. injection Eq; intros; subst. assumption.
+Qed.
+(***** not part of the API *****)
 
-Lemma trees_contain_trees_lookup_2 it tr blk tg :
-  trees_lookup tr blk tg it → trees_contain tg tr blk.
+
+
+Lemma trees_contain_trees_lookup_1 trs ev1 ev2 blk tg :
+  wf_trees trs ev1 ev2 →
+  trees_contain tg trs blk → ∃ it, trees_lookup trs blk tg it.
 Proof.
-Admitted.
+  intros wf.
+  rewrite /trees_contain /trees_lookup /trees_at_block.
+  specialize (wf blk).
+  destruct (trs !! blk) as [tr|]; [|tauto].
+  intros Ex.
+  destruct (wf tr ltac:(reflexivity) tg Ex) as [it [Unq [Det _]]].
+  exists it, tr.
+  split; [|split].
+  - reflexivity.
+  - assumption.
+  - assumption.
+Qed.
+
+Lemma trees_contain_trees_lookup_2 it trs blk tg :
+  trees_lookup trs blk tg it → trees_contain tg trs blk.
+Proof.
+  rewrite /trees_lookup /trees_contain /trees_at_block.
+  destruct (trs !! blk); [|intro H; destruct H as [?[??]]; discriminate].
+  intro H. destruct H as [?[Eqt Lookup]].
+  injection Eqt; intros; subst.
+  apply Lookup.
+Qed.
 
 Lemma apply_trees_access_lookup_same_tag cids ev1 ev2 trs kind blk off1 sz offi t trs':
   apply_within_trees (memory_access kind cids t (off1, sz)) blk trs = Some trs' →
@@ -33,7 +64,11 @@ Lemma apply_trees_access_lookup_same_tag cids ev1 ev2 trs kind blk off1 sz offi 
                  apply_access_perm kind This (bool_decide (protector_is_active itnew.(iprot) cids)) permold = Some permnew.
 Admitted.
 
-Axiom trees_rel_dec : trees → block → tag → tag → rel_pos.
+Definition trees_rel_dec (trs : trees) blk tg tg' :=
+  match trs !! blk with
+  | None => Cousin
+  | Some tr => rel_dec tr tg tg'
+  end.
 
 Lemma apply_trees_access_lookup_general cids ev1 ev2 trs kind blk off1 sz offi acc_tg lu_tg trs' itold :
   apply_within_trees (memory_access kind cids acc_tg (off1, sz)) blk trs = Some trs' →
@@ -45,4 +80,43 @@ Lemma apply_trees_access_lookup_general cids ev1 ev2 trs kind blk off1 sz offi a
                  initp itold = initp itnew ∧
                  iprot itold = iprot itnew ∧
                  apply_access_perm kind (trees_rel_dec trs blk acc_tg lu_tg) (bool_decide (protector_is_active itnew.(iprot) cids)) permold = Some permnew.
-Admitted.
+Proof.
+  intros App wf InBounds Lookup.
+  rewrite /apply_within_trees in App.
+  rewrite bind_Some in App.
+  destruct App as [tr [trSome Acc]].
+  rewrite bind_Some in Acc.
+  destruct Acc as [tr' [Acc Out]].
+  injection Out; intros; subst; clear Out.
+  assert (tree_contains lu_tg tr) as Ex. {
+    eapply trees_at_block_projection; [|eassumption].
+    eapply trees_contain_trees_lookup_2.
+    eassumption.
+  }
+  assert (tree_item_determined lu_tg itold tr) as Det. {
+    destruct Lookup as [trbis [trsLookup trLookup]].
+    assert (trbis = tr) by congruence. subst.
+    apply trLookup.
+  }
+  destruct (apply_access_spec_per_node Ex Det Acc) as [it' [itAcc [Ex' Det']]].
+  exists it'.
+  split; [|split; [|split]].
+  - exists tr'. split; [apply lookup_insert|]. split; assumption.
+  - eapply item_apply_access_preserves_metadata.
+    symmetry. eassumption.
+  - eapply item_apply_access_preserves_metadata.
+    symmetry. eassumption.
+  - rewrite /item_apply_access in itAcc.
+    symmetry in itAcc. rewrite bind_Some in itAcc.
+    destruct itAcc as [perms' [perms'Spec Same]].
+    injection Same; intros; subst; clear Same.
+    pose proof (mem_apply_range'_spec _ _ offi _ _ perms'Spec) as ThisLocation.
+    destruct (decide _); [|unfold range'_contains in *; simpl in *; lia].
+    destruct ThisLocation as [perm [permSome permAcc]].
+    simpl.
+    rewrite /trees_rel_dec trSome.
+    assert (itag itold = lu_tg). { eapply tree_determined_specifies_tag; [|eassumption]; assumption. }
+    subst.
+    rewrite permAcc.
+    rewrite /item_lookup /= permSome //=.
+Qed.
